src/lake/Lake/Load/Workspace.lean
@@ -28,20 +28,20 @@ Does not resolve dependencies.
 -/
 private def loadWorkspaceRoot (config : LoadConfig) : LogIO Workspace := do
   Lean.searchPathRef.set config.lakeEnv.leanSearchPath
-  let (⟨root, wsIdx_eq⟩, env?) ← loadPackageCore "[root]" {config with pkgIdx := 0}
+  let config := {config with pkgIdx := 0}
+  let fileCfg ← loadConfig "[root]" config
+  let root := mkPackage config fileCfg
   let root := {root with outputsRef? := ← CacheRef.mk}
+  let facetConfigs := fileCfg.facetDecls.foldl (·.insert ·.config) initFacetConfigs
   let ws : Workspace := {
     root
     lakeEnv := config.lakeEnv
     lakeArgs? := config.lakeArgs?
-    facetConfigs := initFacetConfigs
+    facetConfigs
     packages_wsIdx h := by simp at h
   }
-  let ws := ws.addPackage' root wsIdx_eq
-  if let some env := env? then
-    IO.ofExcept <| ws.addFacetsFromEnv env config.leanOpts
-  else
-    return ws
+  let ws := ws.addPackage' root wsIdx_mkPackage
+  return ws
 
 /--
 Load a `Workspace` for a Lake package by
